feat: add `RTYPEW` operations for `ADDW`, `SUBW`, `SLLW`, `SRLW`, `SRAW` (#11)
We add the semantics of `rtypew` operations:
- [`addw`](https://msyksphinz-self.github.io/riscv-isadoc/#_addw)
- [`subw`](https://msyksphinz-self.github.io/riscv-isadoc/#_subw)
- [`sllw`](https://msyksphinz-self.github.io/riscv-isadoc/#_sllw)
- [`srlw`](https://msyksphinz-self.github.io/riscv-isadoc/#_srlw)
- [`sraw`](https://msyksphinz-self.github.io/riscv-isadoc/#_sraw)

and we prove their correctness against the Sail specification. 

Co-authored-by: Sarah Kuhn <kuhnsa@student.ethz.ch>

RISCV/Instructions.lean
@@ -65,3 +65,55 @@ def srliw (shamt : BitVec 6) (rs1_val : BitVec 64)  : BitVec 64 :=
 -/
 def sraiw (shamt : BitVec 5) (rs1_val : BitVec 64) : BitVec 64 :=
   BitVec.signExtend 64 (BitVec.sshiftRight' (BitVec.extractLsb 31 0 rs1_val) shamt)
+
+/--
+  Adds the 32-bit of registers rs1 and 32-bit of register rs2 and stores the result in rd.
+  Arithmetic overflow is ignored and the low 32-bits of the result is sign-extended to 64-bits and
+  written to the destination register.
+-/
+def addw (rs2_val : BitVec 64) (rs1_val : BitVec 64) : BitVec 64 :=
+  let rs1 := BitVec.extractLsb' 0 32 rs1_val
+  let rs2 := BitVec.extractLsb' 0 32 rs2_val
+  BitVec.signExtend 64 (BitVec.add rs1 rs2)
+
+/--
+  Subtract the 32-bit of registers rs1 and 32-bit of register rs2 and stores the result in rd.
+  Arithmetic overflow is ignored and the low 32-bits of the result is sign-extended to 64-bits and
+  written to the destination register.
+-/
+def subw (rs2_val : BitVec 64) (rs1_val : BitVec 64) : BitVec 64 :=
+  let rs1 := BitVec.extractLsb' 0 32 rs1_val
+  let rs2 := BitVec.extractLsb' 0 32 rs2_val
+  BitVec.signExtend 64 (BitVec.sub rs1 rs2)
+
+/--
+  Performs logical left shift on the low 32-bits value in register rs1 by the shift amount held in
+  the lower 5 bits of register rs2 and produce 32-bit results and written to the destination
+  register rd.
+-/
+def sllw (rs2_val : BitVec 64) (rs1_val : BitVec 64) : BitVec 64 :=
+  let rs1 := BitVec.extractLsb' 0 32 rs1_val;
+  let rs2 := BitVec.extractLsb' 0 32 rs2_val;
+  let shamt := BitVec.extractLsb' 0 5 rs2;
+  BitVec.signExtend 64 (rs1 <<< shamt)
+
+/--
+  Performs logical right shift on the low 32-bits value in register rs1 by the shift amount held in
+  the lower 5 bits of register rs2 and produce 32-bit results and written to the destination
+  register rd.
+-/
+def srlw (rs2_val : BitVec 64) (rs1_val : BitVec 64)  : BitVec 64 :=
+  let rs1 := BitVec.extractLsb' 0 32 rs1_val;
+  let rs2 := BitVec.extractLsb' 0 32 rs2_val;
+  let shamt := BitVec.extractLsb' 0 5 rs2;
+  BitVec.signExtend 64 (rs1 >>> shamt)
+
+/--
+  Performs arithmetic right shift on the low 32-bits value in register rs1 by the shift amount held
+  in the lower 5 bits of register rs2 and produce 32-bit results and written to the destination
+  register rd.
+-/
+def sraw (rs2_val : BitVec 64) (rs1_val : BitVec 64) :=
+  let rs1 := BitVec.extractLsb 31 0 rs1_val
+  let rs2 := BitVec.extractLsb 4 0 rs2_val
+  BitVec.signExtend 64 (BitVec.sshiftRight' rs1 rs2)
