RISCV/SailPure.lean
@@ -32,3 +32,15 @@ def shiftiwop (shamt : BitVec 5) (op : sopw) (rs1_val : BitVec 64) : BitVec 64 :
     | sopw.SRLIW => (Sail.shift_bits_right rs1_val32 shamt)
     | sopw.SRAIW => (shift_bits_right_arith rs1_val32 shamt)
   (sign_extend (m := ((2 ^i 3) *i 8)) result)
+
+def rtypew (op : ropw) (rs2_val : BitVec 64) (rs1_val : BitVec 64) : BitVec 64 :=
+  let rs1_val32 := Sail.BitVec.extractLsb rs1_val 31 0
+  let rs2_val32 :=  Sail.BitVec.extractLsb rs2_val 31 0
+  let result : (BitVec 32) :=
+    match op with
+    | ropw.ADDW => (rs1_val32 + rs2_val32)
+    | ropw.SUBW => (rs1_val32 - rs2_val32)
+    | ropw.SLLW => (Sail.shift_bits_left rs1_val32 (Sail.BitVec.extractLsb rs2_val32 4 0))
+    | ropw.SRLW => (Sail.shift_bits_right rs1_val32 (Sail.BitVec.extractLsb rs2_val32 4 0))
+    | ropw.SRAW => (shift_bits_right_arith rs1_val32 (Sail.BitVec.extractLsb rs2_val32 4 0))
+  ((sign_extend (m := ((2 ^i 3) *i 8)) result))
